theories/tree_borrows/step_laws/steps_retag.v
@@ -110,7 +110,7 @@ Proof.
   setoid_rewrite trees_equal_same_tags in Hntinmid_t. 2: done.
   clear Hstrs1_eq. (* TODO refactor the above into a separate lemma, maybe? *)
 
-  iDestruct "Hbor" as "(%M_call & %M_tag & %M_t & %M_s & (Hc & Htag_auth & Htag_t_auth & Htag_s_auth) & Hpub_cid & #Hsrel & %Hcall_interp & %Htag_interp & _ & _)".
+  iDestruct "Hbor" as "(%M_call & %M_tag & %M_t & %M_s & (Hc & Htag_auth & Htag_t_auth & Htag_s_auth) & Htainted & Hpub_cid & #Hsrel & %Hcall_interp & %Htag_interp & _ & _)".
   iDestruct (tkmap_lookup with "Htag_auth Hotpub") as "%Hotpub".
   assert (M_tag !! snp σ_s = None) as Htagfresh.
   { destruct (M_tag !! σ_s.(snp)) as [[x []]|] eqn:Heq; last done.
@@ -168,7 +168,13 @@ Proof.
   iFrame "HP_t HP_s". rewrite -Hsnp_eq. iFrame "Hsim". simpl.
   iSplit; last done.
   iExists _, _, _, _. rewrite /bor_interp_inner. iFrame "Htag_auth Htag_t_auth Htag_s_auth Hc". simpl.
-  iSplit; last iSplit; last iSplit; last iSplit; last iSplit.
+  iSplitL "Htainted"; last iSplit; last iSplit; last iSplit; last iSplit; last iSplit.
+  - iDestruct "Htainted" as "(%M&Ht1&Ht2)". iExists M. iFrame "Ht1".
+    iIntros (t' l' Htl'). iDestruct ("Ht2" $! t' l' Htl') as "($&%Ht2)". iPureIntro.
+    simpl. eapply disabled_tag_tree_apply_access_irreversible. 4: done. 2: done. 2: by eapply Hwf_mid_s.
+    eapply disabled_tag_create_child_irreversible. 4: eapply Happly1_s. 2: done.
+    + destruct Ht2 as (Hlt&Ht2); lia.
+    + destruct Ht2 as (Hlt&Ht2); split; last done. lia.
   - iApply pub_cid_interp_preserve_sub. 5: iFrame.
     1,3: by subst σ_t'. all: done.
   - subst σ_t'. rewrite -Hsnp_eq. do 5 (iSplit; first done). simpl.
@@ -344,7 +350,7 @@ Proof.
   setoid_rewrite trees_equal_same_tags in Hntinmid_t. 2: done.
   clear Hstrs1_eq. (* TODO refactor the above into a separate lemma, maybe? *)
 
-  iDestruct "Hbor" as "(%M_call & %M_tag & %M_t & %M_s & (Hc & Htag_auth & Htag_t_auth & Htag_s_auth) & Hpub_cid & #Hsrel & %Hcall_interp & %Htag_interp & _ & _)".
+  iDestruct "Hbor" as "(%M_call & %M_tag & %M_t & %M_s & (Hc & Htag_auth & Htag_t_auth & Htag_s_auth) & Htainted & Hpub_cid & #Hsrel & %Hcall_interp & %Htag_interp & _ & _)".
   iDestruct (tkmap_lookup with "Htag_auth Hotpub") as "%Hotpub".
   assert (M_tag !! snp σ_s = None) as Htagfresh.
   { destruct (M_tag !! σ_s.(snp)) as [[x []]|] eqn:Heq; last done.
@@ -409,7 +415,13 @@ Proof.
   iFrame "HP_t HP_s". rewrite -Hsnp_eq. iFrame "Hsim". simpl.
   iSplit; last done.
   iExists _, _, _, _. rewrite /bor_interp_inner. iFrame "Htag_auth Htag_t_auth Htag_s_auth Hc". simpl.
-  iSplit; last iSplit; last iSplit; last iSplit; last iSplit.
+  iSplitL "Htainted"; last iSplit; last iSplit; last iSplit; last iSplit; last iSplit.
+  - iDestruct "Htainted" as "(%MX&Ht1&Ht2)". iExists MX. iFrame "Ht1".
+    iIntros (t' l' Htl'). iDestruct ("Ht2" $! t' l' Htl') as "($&%Ht2)". iPureIntro.
+    simpl. eapply disabled_tag_tree_apply_access_irreversible. 4: done. 2: done. 2: by eapply Hwf_mid_s.
+    eapply disabled_tag_create_child_irreversible. 4: eapply Happly1_s. 2: done.
+    + destruct Ht2 as (Hlt&Ht2); lia.
+    + destruct Ht2 as (Hlt&Ht2); split; last done. lia.
   - iApply pub_cid_interp_preserve_sub. 5: iFrame.
     1,3: by subst σ_t'. all: done.
   - subst σ_t'. rewrite -Hsnp_eq. do 5 (iSplit; first done). simpl.
@@ -603,7 +615,7 @@ Proof.
   setoid_rewrite trees_equal_same_tags in Hntinmid_t. 2: done.
   clear Hstrs1_eq. (* TODO refactor the above into a separate lemma, maybe? *)
 
-  iDestruct "Hbor" as "(%M_call & %M_tag & %M_t & %M_s & (Hc & Htag_auth & Htag_t_auth & Htag_s_auth) & Hpub_cid & #Hsrel & %Hcall_interp & %Htag_interp & _ & _)".
+  iDestruct "Hbor" as "(%M_call & %M_tag & %M_t & %M_s & (Hc & Htag_auth & Htag_t_auth & Htag_s_auth) & Htainted & Hpub_cid & #Hsrel & %Hcall_interp & %Htag_interp & _ & _)".
   iDestruct (tkmap_lookup with "Htag_auth Hotpub") as "%Hotpub".
   assert (M_tag !! snp σ_s = None) as Htagfresh.
   { destruct (M_tag !! σ_s.(snp)) as [[x []]|] eqn:Heq; last done.
@@ -658,7 +670,13 @@ Proof.
   iFrame "HP_t HP_s". rewrite -Hsnp_eq. iFrame "Hsim". simpl.
   iSplit; last done.
   iExists _, _, _, _. rewrite /bor_interp_inner. iFrame "Htag_auth Htag_t_auth Htag_s_auth Hc". simpl.
-  iSplit; last iSplit; last iSplit; last iSplit; last iSplit.
+  iSplitL "Htainted"; last iSplit; last iSplit; last iSplit; last iSplit; last iSplit.
+  - iDestruct "Htainted" as "(%M&Ht1&Ht2)". iExists M. iFrame "Ht1".
+    iIntros (t' l' Htl'). iDestruct ("Ht2" $! t' l' Htl') as "($&%Ht2)". iPureIntro.
+    simpl. eapply disabled_tag_tree_apply_access_irreversible. 4: done. 2: done. 2: by eapply Hwf_mid_s.
+    eapply disabled_tag_create_child_irreversible. 4: eapply Happly1_s. 2: done.
+    + destruct Ht2 as (Hlt&Ht2); lia.
+    + destruct Ht2 as (Hlt&Ht2); split; last done. lia.
   - iApply pub_cid_interp_preserve_sub. 5: iFrame.
     1,3: by subst σ_t'. all: done.
   - subst σ_t'. rewrite -Hsnp_eq. do 5 (iSplit; first done). simpl.
